LocallyNameless/Confluence.v
@@ -1,0 +1,820 @@
+From FormalSystems Require Export LocallyNameless.STLC.
+
+(* * Confluence *)
+
+(* ** Contraction *)
+
+Inductive FullContraction : Tm -> Tm -> Prop :=
+| FullContraction_app_abs :
+  forall (t1 t2 : Tm) (l : list Atom)
+    (Hlc1 : forall x : Atom, x # l -> lc (t1 {{ 0 ~> x }}))
+    (Hlc2 : lc t2),
+    FullContraction (app (abs t1) t2) (t1 {[ 0 ~> t2 ]}).
+
+#[export] Hint Constructors FullContraction : core.
+
+Lemma lc_FullContraction_l :
+  forall t t' : Tm,
+    FullContraction t t' -> lc t.
+Proof.
+  now inversion 1; subst; econstructor; eauto.
+Qed.
+
+Lemma lc_FullContraction_r :
+  forall t t' : Tm,
+    FullContraction t t' -> lc t'.
+Proof.
+  inversion 1; subst; try (now auto); try (now apply lc_open'; eauto).
+Qed.
+
+#[export] Hint Resolve lc_FullContraction_l lc_FullContraction_r : core.
+
+Lemma FullContraction_det :
+  forall t t1 t2 : Tm,
+    FullContraction t t1 -> FullContraction t t2 -> t1 = t2.
+Proof.
+  now induction 1; inversion 1; eauto.
+Qed.
+
+Lemma FullContraction_subst :
+  forall (t t' u : Tm) (x : Atom),
+    lc u ->
+    FullContraction t t' ->
+    FullContraction (t [[ x := u ]]) (t' [[ x := u]]).
+Proof.
+  inversion 2; cbn.
+  rewrite open'_subst by easy.
+  constructor 1 with (x :: l); [| now apply lc_subst].
+  intros y Hy.
+  rewrite subst_open; [| now firstorder | now eauto].
+  apply lc_subst; [| easy].
+  apply Hlc1.
+  now solve_fresh.
+Qed.
+
+#[export] Hint Resolve FullContraction_det FullContraction_subst : core.
+
+Inductive FullStep : Tm -> Tm -> Prop :=
+| FullStep_FullContraction :
+  forall t t' : Tm,
+    FullContraction t t' ->
+    FullStep t t'
+| FullStep_abs :
+  forall (t t' : Tm) (l : list Atom)
+    (Hfs' : forall x : Atom, x # l -> FullStep (t {{ 0 ~> x }}) (t' {{ 0 ~> x }})),
+    FullStep (abs t) (abs t')
+| FullStep_app_l :
+  forall (t1 t1' t2 : Tm),
+    lc t2 ->
+    FullStep t1 t1' ->
+    FullStep (app t1 t2) (app t1' t2)
+| FullStep_app_r :
+  forall (t1 t1 t2 t2' : Tm),
+    lc t1 ->
+    FullStep t2 t2' ->
+    FullStep (app t1 t2) (app t1 t2').
+
+#[export] Hint Constructors FullStep : core.
+
+Lemma lc_FullStep_l :
+  forall t t' : Tm,
+    FullStep t t' -> lc t.
+Proof.
+  now induction 1; eauto.
+Qed.
+
+Lemma lc_FullStep_r :
+  forall t t' : Tm,
+    FullStep t t' -> lc t'.
+Proof.
+  now induction 1; eauto.
+Qed.
+
+#[export] Hint Resolve lc_FullStep_l lc_FullStep_r : core.
+
+Lemma FullStep_subst :
+  forall (t t' u : Tm) (x : Atom),
+    lc u ->
+    FullStep t t' ->
+    FullStep (t [[ x := u ]]) (t' [[ x := u]]).
+Proof.
+  intros t t' u x Hlc Hfs; revert u x Hlc.
+  induction Hfs; cbn; intros.
+  - constructor.
+    now apply FullContraction_subst.
+  - constructor 2 with (x :: l); intros y Hy.
+    rewrite !subst_open by firstorder.
+    apply H; [| easy].
+    now solve_fresh.
+  - now constructor 3; eauto.
+  - now constructor 4; eauto.
+Qed.
+
+Lemma FullStep_rename :
+  forall (t t' : Tm) (i : nat) (x y : Atom),
+    x # fv t ++ fv t' ->
+    FullStep (t {{ i ~> x }}) (t' {{ i ~> x }}) ->
+      FullStep (t {{ i ~> y }}) (t' {{ i ~> y }}).
+Proof.
+  intros t t' i x y Hx Hfs.
+  rewrite <- 2!open'_atom.
+  rewrite 2!open'_spec with (x := x) by solve_fresh.
+  now apply FullStep_subst.
+Qed.
+
+#[export] Hint Resolve FullStep_subst FullStep_rename : core.
+
+Inductive MultiStep : Tm -> Tm -> Prop :=
+| MultiStep_refl :
+  forall (t : Tm),
+    lc t ->
+    MultiStep t t
+| MultiStep_step_trans :
+  forall (t1 t2 t3 : Tm),
+    FullStep t1 t2 ->
+    MultiStep t2 t3 ->
+    MultiStep t1 t3.
+
+#[export] Hint Constructors MultiStep : core.
+
+Require Import Coq.Classes.RelationClasses.
+
+#[export] Instance Transitive_MultiStep : Transitive MultiStep.
+Proof.
+  now induction 1; eauto.
+Qed.
+
+Require Import Coq.Relations.Relation_Operators.
+
+Lemma lc_MultiStep_l :
+  forall t t' : Tm,
+    MultiStep t t' -> lc t.
+Proof.
+  now induction 1; eauto.
+Qed.
+
+Lemma lc_MultiStep_r :
+  forall t t' : Tm,
+    MultiStep t t' -> lc t'.
+Proof.
+  now induction 1; eauto.
+Qed.
+
+#[export] Hint Resolve lc_MultiStep_l lc_MultiStep_r : core.
+
+Lemma MultiStep_subst :
+  forall (t t' u : Tm) (x : Atom),
+    lc u ->
+    MultiStep t t' ->
+    MultiStep (t [[ x := u ]]) (t' [[ x := u]]).
+Proof.
+  intros t t' u x Hlc Hms; revert u x Hlc.
+  induction Hms; cbn; intros; [now eauto |].
+  constructor 2 with (t2 [[ x := u ]]).
+  - now apply FullStep_subst.
+  - now apply IHHms.
+Restart.
+  now induction 2; eauto.
+Qed.
+
+Lemma MultiStep_rename :
+  forall (t t' : Tm) (i : nat) (x y : Atom),
+    x # fv t ++ fv t' ->
+    MultiStep (t {{ i ~> x }}) (t' {{ i ~> x }}) ->
+      MultiStep (t {{ i ~> y }}) (t' {{ i ~> y }}).
+Proof.
+  intros t t' i x y Hx Hfs.
+  rewrite <- 2!open'_atom.
+  rewrite 2!open'_spec with (x := x) by solve_fresh.
+  now apply MultiStep_subst.
+Qed.
+
+#[export] Hint Resolve MultiStep_subst MultiStep_rename : core.
+
+Lemma MultiStep_FullStep :
+  forall t1 t2 : Tm,
+    FullStep t1 t2 -> MultiStep t1 t2.
+Proof.
+  now eauto.
+Qed.
+
+Lemma MultiStep_abs :
+  forall t t' : Tm,
+    (exists l : list Atom, forall x : Atom, x # l ->
+      MultiStep (t {{ 0 ~> x }}) (t' {{ 0 ~> x }})) ->
+        MultiStep (abs t) (abs t').
+Proof.
+  intros t t' [l Hms].
+  pose (x := fresh (l ++ fv t ++ fv t')).
+  specialize (Hms x ltac:(subst x; solve_fresh)) as Hms'.
+  clearbody x.
+  remember (t {{ 0 ~> x }}) as u.
+  remember (t' {{ 0 ~> x }}) as u'.
+  clear Hms.
+  revert t t' Hequ Hequ'.
+  induction Hms'; intros; subst.
+  - replace (abs t') with (abs t0).
+    + apply MultiStep_refl.
+      apply lc_abs with l; intros y Hy.
+      now apply lc_open_invariant with x.
+    + admit.
+  - constructor 2 with (abs (t2 {{ 0 <~ x }})).
+    + constructor 2 with l. 
+      intros y Hy.
+      admit.
+    + apply IHHms'; [| easy].
+      
+specialize (IHHms' (t2 {{ 0 <~ x }}) t').
+Admitted.
+
+Lemma MultiStep_abs' :
+  forall t t' : Tm,
+    MultiStep t t' -> MultiStep (abs t) (abs t').
+Proof.
+  induction 1.
+  - apply MultiStep_refl.
+    now apply lc_abs with []; eauto.
+  - transitivity (abs t2); [| easy].
+    apply MultiStep_FullStep.
+    apply FullStep_abs with []; intros x _.
+    now rewrite 2!open_lc by eauto.
+Qed.
+
+Lemma MultiStep_app_l :
+  forall t1 t1' t2 : Tm,
+    lc t2 ->
+    MultiStep t1 t1' ->
+    MultiStep (app t1 t2) (app t1' t2).
+Proof.
+  now induction 2; eauto.
+Qed.
+
+Lemma MultiStep_app_r :
+  forall t1 t2 t2' : Tm,
+    lc t1 ->
+    MultiStep t2 t2' ->
+    MultiStep (app t1 t2) (app t1 t2').
+Proof.
+  now induction 2; eauto.
+Qed.
+
+Lemma MultiStep_app :
+  forall t1 t1' t2 t2' : Tm,
+    MultiStep t1 t1' ->
+    MultiStep t2 t2' ->
+    MultiStep (app t1 t2) (app t1' t2').
+Proof.
+  induction 2.
+  - now apply MultiStep_app_l.
+  - transitivity (app t1 t2); [| easy].
+    apply MultiStep_app_r; [| now eauto].
+    now apply lc_MultiStep_l in H.
+Qed.
+
+#[export] Hint Resolve
+  MultiStep_FullStep
+  MultiStep_abs MultiStep_abs'
+  MultiStep_app_l MultiStep_app_r MultiStep_app
+    : core.
+
+Inductive ParallelStep : Tm -> Tm -> Prop :=
+| ParallelStep_fvar :
+  forall (x : Atom),
+    ParallelStep x x
+| ParallelStep_abs :
+  forall (t1 t2 : Tm) (l : list Atom)
+    (Hps' : forall x : Atom, x # l -> ParallelStep (t1 {{ 0 ~> x }}) (t2 {{ 0 ~> x }})),
+    ParallelStep (abs t1) (abs t2)
+| ParallelStep_app :
+  forall (t1 t1' t2 t2' : Tm),
+    ParallelStep t1 t1' ->
+    ParallelStep t2 t2' ->
+    ParallelStep (app t1 t2) (app t1' t2')
+| ParallelStep_app_abs :
+  forall (t1 t1' t2 t2' : Tm) (l : list Atom)
+    (Hps1 : forall x : Atom, x # l -> ParallelStep (t1 {{ 0 ~> x }}) (t1' {{ 0 ~> x }}))
+    (Hps2 : ParallelStep t2 t2'),
+    ParallelStep (app (abs t1) t2) (t1' {[ 0 ~> t2' ]}).
+
+#[export] Hint Constructors ParallelStep : core.
+
+Lemma ParallelStep_refl :
+  forall t : Tm,
+    lc t ->
+    ParallelStep t t.
+Proof.
+  induction 1; eauto.
+Admitted.
+
+Lemma lc_ParallelStep_l :
+  forall t t' : Tm,
+    ParallelStep t t' -> lc t.
+Proof.
+  now induction 1; eauto.
+Qed.
+
+Lemma lc_ParallelStep_r :
+  forall t t' : Tm,
+    ParallelStep t t' -> lc t'.
+Proof.
+  now induction 1; eauto.
+Qed.
+
+#[export] Hint Resolve ParallelStep_refl lc_ParallelStep_l lc_ParallelStep_r : core.
+
+Lemma ParallelStep_subst :
+  forall (t t' u : Tm) (x : Atom),
+    lc u ->
+    ParallelStep t t' ->
+    ParallelStep (t [[ x := u ]]) (t' [[ x := u]]).
+Proof.
+  intros t t' u x Hlc Hps; revert u x Hlc.
+  induction Hps; cbn; intros.
+  - now decide_all; eauto.
+  - constructor 2 with (x :: l); intros y Hy.
+    rewrite !subst_open by firstorder.
+    apply H; [| easy].
+    now solve_fresh.
+  - now constructor 3; eauto.
+  - rewrite open'_subst by easy.
+    constructor 4 with (x :: l); [| now apply IHHps].
+    intros y Hy.
+    rewrite 2!subst_open by firstorder.
+    now apply H; solve_fresh.
+Qed.
+
+Lemma ParallelStep_rename :
+  forall (t t' : Tm) (i : nat) (x y : Atom),
+    x # fv t ++ fv t' ->
+    ParallelStep (t {{ i ~> x }}) (t' {{ i ~> x }}) ->
+      ParallelStep (t {{ i ~> y }}) (t' {{ i ~> y }}).
+Proof.
+  intros t t' i x y Hx Hfs.
+  rewrite <- 2!open'_atom.
+  rewrite 2!open'_spec with (x := x) by solve_fresh.
+  now apply ParallelStep_subst.
+Qed.
+
+#[export] Hint Resolve ParallelStep_subst ParallelStep_rename : core.
+
+Lemma ParallelStep_FullContraction :
+  forall t1 t2 : Tm,
+    FullContraction t1 t2 -> ParallelStep t1 t2.
+Proof.
+  now inversion 1; subst; eauto.
+Qed.
+
+Lemma ParallelStep_FullStep :
+  forall t1 t2 : Tm,
+    FullStep t1 t2 -> ParallelStep t1 t2.
+Proof.
+  induction 1; eauto.
+  now apply ParallelStep_FullContraction.
+Qed.
+
+Lemma MultiStep_ParallelStep :
+  forall t1 t2 : Tm,
+    ParallelStep t1 t2 -> MultiStep t1 t2.
+Proof.
+  induction 1; eauto.
+  transitivity (app (abs t1') t2); [now eauto |].
+  transitivity (app (abs t1') t2'); [now eauto |].
+  now eauto 7.
+Qed.
+
+#[export] Hint Resolve ParallelStep_FullStep MultiStep_ParallelStep : core.
+
+Module development_try1.
+
+Fixpoint development (t : Tm) : Tm :=
+match t with
+| fvar x          => fvar x
+| bvar i          => bvar i
+| abs t'          => abs (development t' {{ 0 ~> fresh (fv t') }})
+| app (abs t1) t2 => development t1 {[ 0 ~> development t2 ]}
+| app t1 t2       => app (development t1) (development t2)
+| _               => unit
+end.
+
+Lemma development_open :
+  forall (t : Tm) (i : nat) (a : Atom),
+    lc t ->
+    development t {{ i ~> a }} = development (t {{ i ~> a }}).
+Proof.
+  intros.
+  rewrite (open_lc t i a) by easy.
+Abort.
+
+Lemma lc_development :
+  forall (t : Tm),
+    lc t -> lc (development t).
+Proof.
+  induction 1; cbn; auto.
+  - admit.
+Abort.
+
+End development_try1.
+
+Module development_try2.
+
+Unset Guard Checking.
+Fixpoint development (t : Tm) : Tm :=
+match t with
+| fvar x          => fvar x
+| bvar i          => bvar i
+| abs t'          => abs (development t')
+| app (abs t1) t2 =>
+  let x := fresh (fv t1) in
+    development (t1 {{ 0 ~> x }}) [[ x := development t2 ]]
+| app t1 t2       => app (development t1) (development t2)
+| _               => unit
+end.
+Set Guard Checking.
+
+Lemma development_open :
+  forall (t : Tm) (i : nat) (a : Atom),
+    development t {{ i ~> a }} = development (t {{ i ~> a }}).
+Proof.
+  induction t; cbn; intros; auto.
+  - now decide_all.
+  - now rewrite IHt.
+  - destruct t1; cbn in *; rewrite 1?IHt1, 1?IHt2; auto.
+    + now decide_all.
+    +
+Admitted.
+
+Lemma lc_development :
+  forall (t : Tm),
+    lc t -> lc (development t).
+Proof.
+  induction 1; cbn; auto.
+  - constructor 2 with l; intros x Hx.
+Admitted.
+
+Lemma development_spec :
+  forall t1 t2 : Tm,
+    ParallelStep t1 t2 -> ParallelStep t2 (development t1).
+Proof.
+  intros t1 t2 Hps.
+  assert (lc t2) by eauto.
+  induction Hps; cbn.
+  - now eauto.
+  - apply ParallelStep_abs with l; intros x Hx.
+    now rewrite development_open; eauto.
+  - destruct t1; cbn in *; try now auto.
+    inversion H; subst.
+Admitted.
+
+End development_try2.
+
+Module development_try3.
+
+Unset Guard Checking.
+Fixpoint development (t : Tm) : Tm :=
+match t with
+| fvar x          => fvar x
+| bvar i          => bvar i
+| abs t'          => abs (development t')
+| app (abs t1) t2 =>
+  let x := fresh (fv t1) in
+    development t1 {[ 0 ~> development t2 ]}
+| app t1 t2       => app (development t1) (development t2)
+| _               => unit
+end.
+Set Guard Checking.
+
+Lemma development_open :
+  forall (t : Tm) (i : nat) (a : Atom),
+    development t {{ i ~> a }} = development (t {{ i ~> a }}).
+Proof.
+  induction t; cbn; intros; auto.
+  - now decide_all.
+  - now rewrite IHt.
+  - destruct t1; cbn in *; rewrite 1?IHt1, 1?IHt2; auto.
+    + now decide_all.
+    + injection (IHt1 i a) as [= <-].
+      rewrite <- IHt2.
+Admitted.
+
+Lemma development_spec :
+  forall t1 t2 : Tm,
+    ParallelStep t1 t2 -> ParallelStep t2 (development t1).
+Proof.
+  induction 1; cbn.
+  - now eauto.
+  - apply ParallelStep_abs with l; intros x Hx.
+    now rewrite development_open; auto.
+  - destruct t1; cbn in *; try now auto.
+    inversion H; subst.
+    inversion IHParallelStep1; subst; eauto.
+  - 
+Admitted.
+
+End development_try3.
+
+Module development_try4.
+
+Fixpoint development (i : nat) (t : Tm) : Tm :=
+match t with
+| fvar x          => fvar x
+| bvar j          => bvar j
+| abs t'          => abs (development (S i) t')
+| app (abs t1) t2 => development (S i) t1 {[ 0 ~> development i t2 ]}
+| app t1 t2       => app (development i t1) (development i t2)
+| _               => unit
+end.
+
+End development_try4.
+
+Module development_try5.
+
+Unset Guard Checking.
+Fixpoint development (t : Tm) : Tm :=
+match t with
+| fvar x          => fvar x
+| bvar i          => bvar i
+| abs t'          =>
+  let x := fresh (fv t') in
+    abs (development (t' {{ 0 ~> x }}) {{ 0 <~ x }})
+| app (abs t1) t2 =>
+  let x := fresh (fv t1) in
+    development (t1 {{ 0 ~> x }}) [[ x := development t2 ]]
+| app t1 t2       => app (development t1) (development t2)
+| _               => unit
+end.
+Set Guard Checking.
+
+Lemma development_open :
+  forall (t : Tm) (i : nat) (a : Atom),
+    development t {{ i ~> a }} = development (t {{ i ~> a }}).
+Proof.
+  induction t; cbn; intros i x; try now auto.
+  - now decide_all.
+  - admit.
+  - destruct t1; cbn in *; rewrite 1?IHt1, 1?IHt2; auto.
+    + now decide_all.
+    + 
+Admitted.
+
+Lemma development_spec :
+  forall t1 t2 : Tm,
+    ParallelStep t1 t2 -> ParallelStep t2 (development t1).
+Proof.
+  induction 1; cbn.
+  - now eauto.
+  - apply ParallelStep_abs with l; intros x Hx.
+    apply ParallelStep_rename with (fresh (fv t1 ++ fv t2)).
+Admitted.
+
+End development_try5.
+
+Axiom development : Tm -> Tm.
+
+Axiom development_spec :
+  forall t1 t2 : Tm,
+    ParallelStep t1 t2 -> ParallelStep t2 (development t1).
+
+Lemma confluent_ParallelStep :
+  forall t t1 t2 : Tm,
+    ParallelStep t t1 -> ParallelStep t t2 ->
+      ParallelStep t1 (development t) /\ ParallelStep t2 (development t).
+Proof.
+  intros t t1 t2 Hps1 Hps2.
+  now split; apply development_spec.
+Qed.
+
+Inductive ParallelMultiStep : Tm -> Tm -> Prop :=
+| ParallelMultiStep_refl :
+  forall (t : Tm),
+    lc t ->
+    ParallelMultiStep t t
+| ParallelMultiStep_step_trans :
+  forall (t1 t2 t3 : Tm),
+    ParallelStep t1 t2 ->
+    ParallelMultiStep t2 t3 ->
+    ParallelMultiStep t1 t3.
+
+#[export] Hint Constructors ParallelMultiStep : core.
+
+#[export] Instance Transitive_ParallelMultiStep : Transitive ParallelMultiStep.
+Proof.
+  now induction 1; eauto.
+Qed.
+
+Lemma lc_ParallelMultiStep_l :
+  forall t t' : Tm,
+    ParallelMultiStep t t' -> lc t.
+Proof.
+  now induction 1; eauto.
+Qed.
+
+Lemma lc_ParallelMultiStep_r :
+  forall t t' : Tm,
+    ParallelMultiStep t t' -> lc t'.
+Proof.
+  now induction 1; eauto.
+Qed.
+
+Lemma ParallelMultiStep_ParallelStep :
+  forall t1 t2 : Tm,
+    ParallelStep t1 t2 -> ParallelMultiStep t1 t2.
+Proof.
+  now eauto.
+Qed.
+
+#[export] Hint Resolve
+  lc_ParallelMultiStep_l lc_ParallelMultiStep_r
+  ParallelMultiStep_ParallelStep
+    : core.
+
+Lemma ParallelMultiStep_app_l :
+  forall t1 t1' t2 : Tm,
+    ParallelMultiStep t1 t1' ->
+    lc t2 ->
+      ParallelMultiStep (app t1 t2) (app t1' t2).
+Proof.
+  now induction 1; eauto.
+Qed.
+
+Lemma ParallelMultiStep_app_r :
+  forall t1 t2 t2' : Tm,
+    lc t1 ->
+    ParallelMultiStep t2 t2' ->
+      ParallelMultiStep (app t1 t2) (app t1 t2').
+Proof.
+  now induction 2; eauto.
+Qed.
+
+Lemma ParallelMultiStep_app :
+  forall t1 t1' t2 t2' : Tm,
+    ParallelMultiStep t1 t1' ->
+    ParallelMultiStep t2 t2' ->
+      ParallelMultiStep (app t1 t2) (app t1' t2').
+Proof.
+  intros.
+  transitivity (app t1' t2).
+  - now apply ParallelMultiStep_app_l; eauto.
+  - now apply ParallelMultiStep_app_r; eauto.
+Qed.
+
+#[export] Hint Resolve
+  ParallelMultiStep_app_l ParallelMultiStep_app_r ParallelMultiStep_app
+    : core.
+
+Lemma MultiStep_ParallelMultiStep :
+  forall t1 t2 : Tm,
+    MultiStep t1 t2 <-> ParallelMultiStep t1 t2.
+Proof.
+  split.
+  - now induction 1; eauto.
+  - induction 1; [now eauto |].
+    now transitivity t2; eauto.
+Qed.
+
+Lemma confluent_ParallelStep_ParallelMultiStep :
+  forall t t1 t2 : Tm,
+    ParallelStep t t1 -> ParallelMultiStep t t2 ->
+      exists t3 : Tm, ParallelMultiStep t1 t3 /\ ParallelMultiStep t2 t3.
+Proof.
+  intros t t1 t2 H1 H2; revert t1 H1.
+  induction H2; intros.
+  - now exists t1; eauto.
+  - edestruct (IHParallelMultiStep (development t1)) as [t4 [IH1 IH2] ].
+    + now apply development_spec.
+    + exists t4; split; [| easy].
+      transitivity (development t1); [| easy].
+      now apply ParallelMultiStep_ParallelStep, development_spec.
+Qed.
+
+Lemma confluent_ParallelMultiStep :
+  forall t t1 t2 : Tm,
+    ParallelMultiStep t t1 -> ParallelMultiStep t t2 ->
+      exists t3 : Tm, ParallelMultiStep t1 t3 /\ ParallelMultiStep t2 t3.
+Proof.
+  intros t t1 t2 H1 H2; revert t2 H2.
+  induction H1; intros.
+  - now exists t2; eauto.
+  - destruct (confluent_ParallelStep_ParallelMultiStep _ _ _ H H2) as [t4 [H24 H04] ].
+    edestruct (IHParallelMultiStep _ H24) as [t5 [H35 H45] ].
+    exists t5; split; [easy |].
+    now transitivity t4.
+Qed.
+
+Lemma confluent_Step :
+  forall t t1 t2 : Tm,
+    MultiStep t t1 -> MultiStep t t2 ->
+      exists t3 : Tm, MultiStep t1 t3 /\ MultiStep t2 t3.
+Proof.
+  setoid_rewrite MultiStep_ParallelMultiStep.
+  intros t t1 t2 Hs1 Hs2.
+  now apply confluent_ParallelMultiStep with t.
+Qed.
+
+Inductive Development : Tm -> Tm -> Prop :=
+| Development_fvar :
+  forall (x : Atom),
+    Development x x
+| Development_abs :
+  forall (t1 t2 : Tm) (l : list Atom)
+    (Hps' : forall x : Atom, x # l -> Development (t1 {{ 0 ~> x }}) (t2 {{ 0 ~> x }})),
+    Development (abs t1) (abs t2)
+| Development_app :
+  forall (t1 t1' t2 t2' : Tm),
+    (forall u, t1 <> abs u) ->
+    Development t1 t1' ->
+    Development t2 t2' ->
+    Development (app t1 t2) (app t1' t2')
+| Development_app_abs :
+  forall (t1 t1' t2 t2' : Tm) (l : list Atom)
+    (Hps1 : forall x : Atom, x # l -> Development (t1 {{ 0 ~> x }}) (t1' {{ 0 ~> x }}))
+    (Hps2 : Development t2 t2'),
+    Development (app (abs t1) t2) (t1' {[ 0 ~> t2' ]}).
+
+#[export] Hint Constructors Development : core.
+
+Lemma lc_Development_l :
+  forall t t' : Tm,
+    Development t t' -> lc t.
+Proof.
+  now induction 1; eauto.
+Qed.
+
+Lemma lc_Development_r :
+  forall t t' : Tm,
+    Development t t' -> lc t'.
+Proof.
+  now induction 1; eauto.
+Qed.
+
+#[export] Hint Resolve lc_Development_l lc_Development_r : core.
+
+Lemma Development_det :
+  forall t t1 t2 : Tm,
+    Development t t1 -> Development t t2 -> t1 = t2.
+Proof.
+  intros t t1 t2 Hd1 Hd2; revert t2 Hd2.
+  induction Hd1; inversion 1; subst.
+  - easy.
+  - apply abs_eq with (fresh (l ++ l0 ++ fv t2 ++ fv t4)); [now solve_fresh |].
+    apply H; [now solve_fresh |].
+    apply Hps'0.
+    now solve_fresh.
+  - now erewrite IHHd1_1, IHHd1_2; eauto.
+  - now contradiction (H t3).
+  - now contradiction (H2 t1).
+  - rewrite !(open'_spec _ 0 (fresh (l ++ l0 ++ fv t1' ++ fv t1'0))) by solve_fresh.
+    f_equal; [| now apply IHHd1].
+    apply H; [now solve_fresh |].
+    apply Hps0.
+    now solve_fresh.
+Qed.
+
+Lemma Development_FullContraction :
+  forall t1 t2 t3 : Tm,
+    FullContraction t1 t2 -> Development t2 t3 -> Development t1 t3.
+Proof.
+  do 2 inversion 1; subst.
+  - rewrite H4.
+    constructor 4 with l.
+Admitted.
+
+Lemma FullStep_Development :
+  forall t1 t2 t3 : Tm,
+    FullStep t1 t2 -> Development t2 t3 -> Development t1 t3.
+Proof.
+  intros t1 t2 t3 Hfs Hd; revert t3 Hd.
+  induction Hfs; intros.
+  - now eapply Development_FullContraction; eauto.
+  - inversion Hd; subst.
+    constructor 2 with (l ++ l0); intros x Hx.
+    eapply H; [now solve_fresh |].
+    now apply Hps'; solve_fresh.
+  - inversion Hd; subst.
+    + constructor; [| now auto..].
+      intros u [= ->].
+      inversion Hfs; subst; [now inversion H0 |].
+      now contradiction (H2 t').
+    + inversion Hd; subst.
+      * now contradiction (H3 t0).
+      * 
+Restart.
+  intros t1 t2 t3 Hfs Hd; revert t1 Hfs.
+  induction Hd; intros.
+  - inversion Hfs; inversion H; subst.
+    destruct t0; cbn in H4; inversion H4; subst; cbn.
+    constructor 4 with l. 2: easy.
+intros y Hy.
+  
+Qed.
+
+Lemma MultiStep_Development :
+  forall t1 t2 : Tm,
+    Development t1 t2 -> MultiStep t1 t2.
+Proof.
+  induction 1; eauto.
+  transitivity (app (abs t1') t2); [now eauto |].
+  transitivity (app (abs t1') t2'); [now eauto |].
+  now eauto 7.
+Qed.
+
+#[export] Hint Resolve Development_FullStep MultiStep_Development : core.
